\lesson{21}{di 08 dec 2020 10:38}{}

Recap:

\begin{align*}
    H_0(G, A) &= A_G & H^{0}(G, A) &= A^{G}\\
    H_1(G, \Z) &= \frac{G}{[G,G]} & H^{1}(G, A) &= \frac{\Der(G, A)}{\PDer(G, A)}
.\end{align*}

Remember:
\[
    D(gh) = gD(h) + D(g) \qquad \qquad D_a(g) = ga - a
.\] 

Today: 
\begin{enumerate}[(1)]
    \item Description of free resolution of any group! (Focussing on cohomology)
    \item Interpretation of $H^{2}(G, A)$.
\end{enumerate}

\nsection35{The Bar resolution and Group cohomology}

Let $B^u_n$ the free  $\Z G$-module generated by all elements of the form 
\[
    [g_1 \otimes g_2 \otimes \cdots \otimes g_n] \qquad \text{where } g_i \in G
.\] 
This is just notation, has nothing to do with tensor product!!!! We could just have written $(g_1, g_2, \cdots, g_n)$.

\[
    \to  B^u_3 
    \xrightarrow{d}  B^u_2
    \xrightarrow{d}  B^u_1
    \xrightarrow{d}  B^u_0
    \xrightarrow{\epsilon} \Z
    \to  0
.\] 

\paragraph{What is $\epsilon$}
    $B^u_0$ is the free $\Z G$-module generated by $[]$.
    Then  $ B^u_0 \cong \Z G$.
    \[
        \sum_{g \in G} \alpha_g g []  \longmapsto \sum \alpha_g g
    .\] 

    So we define
    \begin{align*}
        \epsilon: B^u_0 &\longrightarrow \Z  \\
        \sum \alpha_g g [] &\longmapsto \sum \alpha_g
    .\end{align*}

\paragraph{What is $d: B^u_n \to  B^u_{n-1}$}

\[
    d = \sum_{i=0}^{n} (-1)^{i} d_i
.\] 
Each $d_i: B^u_n \to  B^u_{n-1}$ is a $G$-map, so a $\Z G$-morphism.
So it is enough to define it on the generators, $[g_1 \otimes \cdots \otimes g_n]$.

\begin{align*}
    d_0[g_1 \otimes \cdots \otimes g_n] &= g_1 [ g_2 \otimes \cdots \otimes g_n] \in B^u_{n-1}\\
    d_i[g_1 \otimes \cdots \otimes g_n] &= [g_1 \otimes \cdots \otimes g_{i-1} \otimes g_i g_{i+1} \otimes \cdots \otimes g_n] \qquad 1 \le i \le  n-1\\
    d_n[g_1 \otimes \cdots \otimes g_n] &= [g_1 \otimes \cdots \otimes g_{n-1}]
.\end{align*}

\begin{eg}
    What is $d: B^u_1 \to  B^u_0$?. We know that $d = d_0 - d_1$

    \begin{align*}
        d[g_1] &= d_0 [g_1] - d_1[g_1]\\
               &= g_1[\ ] - [\ ]\\
               &= (g_1 - 1)[\ ]
    .\end{align*} 

    What is $d: B^u_2 \to  B^u_1$? We have
    
    \begin{align*}
        d[g_1 \otimes g_2] &= g_1 [g_2] - [g_1 g_2] + [g_1]
    .\end{align*}
    What is $d: B^u_3 \to  B^u_2$? We 
    \begin{align*}
        d[g_1 \otimes g_2 \otimes g_3] &= g_1[g_2 \otimes g_3]\\
                                       &\quad  - [g_1g_2 \otimes g_3]\\
                                       &\quad + [g_1 \otimes g_2 g_3]\\
                                       &\quad - [g_1 \otimes g_2]
    .\end{align*}
\end{eg}        

Now we check that this is indeed a free resolution. So it should be a complex that is exact.

\[
    \to  B^u_3 
    \xrightarrow{d}  B^u_2
    \xrightarrow{d}  B^u_1
    \xrightarrow{d}  B^u_0
    \xrightarrow{\epsilon} \Z
    \to  0
.\] 

First we check that composition is zero.

\begin{itemize}
    \item \[
            (\epsilon d) [g_1] = \epsilon( g_1[] - []) = 1 - 1 = 0
        .\] 
    \item Now, $d^2 = 0$. We will not do this in general.
        We just show an example. $B^u_3 \xrightarrow{d} B^u_2 \xrightarrow{d} B^u_1$.
        Then
        \begin{align*}
            (d  \circ  d) ([g_1 \otimes g_2 \otimes g_3]) &= d(g_1[g_2 \otimes g_3] - [g_1g_2 \otimes g_3] + [g_1 \otimes g_2 g_3] - [g_1 \otimes g_2])\\
                                                          &= g_1 g_2[g_3] - g_1[g_2g_3] + g_1[g_2]\\
                                                          & \quad - g_1 g_2[g_3] + [g_1 g_2 g_3] - [g_1g_2]\\
                                                          & \quad + g_1[g_2g_3] - [g_1g_2g_3] + [g_1]\\
                                                          & \quad - g_1[g_2] + [g_1g_2] - [g_1]\\
                                                          &= 0
        .\end{align*} 
\end{itemize}

This is a complex!

\subsection*{The normalized Bar resolution}

Let $ B_n $ be the free $\Z G$-module on
\[
    [g_1|g_2|\cdots | g_n] \qquad \text{ with } g_i \in  G \setminus \{1\} 
,\] 
so fewer generators.
We still have that $B_0$ is generated by $[]$, so  $\cong \Z G$.

\begin{remark}
    For an infinite group, it may not make a big difference, for a finite group it maybe does.
\end{remark}


\[
    d = \sum_{i=0}^{n} (-1)^{i} d_i
.\] 
Each $d_i: B_n \to  B_{n-1}$ is a $G$-map, so a $\Z G$-morphism.
So it is enough to define it on the generators, $[g_1 | \cdots | g_n]$.

\begin{align*}
    d_0[g_1 | \cdots | g_n] &= g_1 [ g_2 | \cdots | g_n] \in B^u_{n-1}\\
    d_i[g_1 | \cdots | g_n] &=
    \begin{cases}
        [g_1 | \cdots | g_{i-1} | g_i g_{i+1} | \cdots | g_n]  & g_i g_{i+1} \neq 1\\
        0 & \text{else} \\
    \end{cases}
\qquad 1 \le i \le  n-1
    \\
    d_n[g_1 | \cdots | g_n] &= [g_1 | \cdots | g_{n-1}]
.\end{align*}

To make this easier, especially the cases, we have a convention:

\[
    [g_1 | g_2 \cdots | g_n] = 0  \qquad \text{if some $g_i = 1$}
,\] 
then the formulas stay the same as before!

\begin{theorem}[6.5.3]
    \[
        \to  B^u_3 
        \xrightarrow{d}  B^u_2
        \xrightarrow{d}  B^u_1
        \xrightarrow{d}  B^u_0
        \xrightarrow{\epsilon} \Z
        \to  0 \tag{$*$}
    ,\] 
    and the normalized one is a free resolution of $\Z$. (The sequence is exact)
\end{theorem}
\begin{proof}
    We already know that $*$ is a chain complex.
    It is enough to prove that $H_n(-)= 0$ for the chain complex.
    For this we can construct a contracting homotopy.
Recall:
\begin{definition}
Contracting homotopy is a 
\[
    \begin{tikzcd}
        B^u_3 \arrow[r, ""] 
        &B^u_2 \arrow[r, ""]  \arrow[dl, "s_2"] \arrow[d, "\operatorname{Id}"]
        &B^u_1 \arrow[r, ""] \arrow[dl, "s_1"] \arrow[d, "\operatorname{Id}"]
        &B^u_0 \arrow[r, ""] \arrow[dl, "s_0"] \arrow[d, "\operatorname{Id}"]
        &\Z \arrow[r, ""] \arrow[dl, "s_{-1}"]
        &0 \arrow[r, ""] \arrow[dl, "s_{-2}"]
        &0 \\
        B^u_3 \arrow[r, ""]
        &B^u_2 \arrow[r, ""]
        &B^u_1 \arrow[r, ""]
        &B^u_0 \arrow[r, ""]
        &\Z \arrow[r, ""]
        &0 \arrow[r, ""]
        &0 
    \end{tikzcd}
\]
such that the Identity map is null homotopic. 
So then identity map induces zero map on homology, so zero map is identity map, so homology is zero.
\end{definition}
This are $\Z G$ complexes. So we need to find $G$-maps.
But we can also look at this complex as a complex of $\Z$-modules.
So enough to find $s_i$ that are $\Z$-morphisms,  i.e. morphisms of abelian groups.
That's enough.
Because then this proves homology of this $\Z$-complex is zero. But homology is still just kernel divided by image, and these kernels and images don't change if we consider these modules as $\Z G$ modules or as $\Z$-modules.

Note: Elements of $B_n^{u}$ can be written as  $\Z G$ linear combinations of $[g_1 \otimes g_2 \cdots \otimes g_n]$.
So they can also be written uniquely as $\Z$-linear combinations of elements of the form 
\[
    g_0[g_1 \otimes g_2 \cdots g_n]
.\] 
Conclusion: $B_n^{u}$ is the free abelian group on these kind of elements.
So enough to specify what $s_i$ does on these kind of elements.

 \begin{align*}
     s_{-1}&: \Z \to  B_0: 1 \mapsto [\ ]\\
    s_{n}&: B^{u}_n \to  B_{n+1}^{u}: g_0[g_1 \otimes \cdots \otimes g_n] \mapsto [g_0 \otimes g_1 \cdots \otimes g_n]
.\end{align*} 

We should check this first on special cases on right of diagram (do this yourself)
Let us check the general case

\[
    \begin{tikzcd}
        B^u_{n+1} \arrow[r, ""]
        & B^u_{n} \arrow[dl, "s_{n-1}"]\arrow[r, "d"] \arrow[d, "\operatorname{Id}"]
        & B^u_{n-1} \arrow[dl, "s_{n-1}"]\\
        B^u_{n+1} \arrow[r, "d"]
        & B^u_{n} \arrow[r, ""]
        & B^u_{n-1}\\
    \end{tikzcd}
\]

\begin{align*}
    (s_{n-1}  \circ  d)(g_0[g_1 \otimes \cdots \otimes g_n]) &= s_{n-1}(g_0 d([g_1 \otimes \cdots \otimes g_n])\\
                                                             &= s_{n-1}(
                                                             g_0 g_1[g_2 \otimes \cdots \otimes g_n]
                                                             - g_0 [g_1 g_2 \otimes \cdots \otimes g_n]
                                                             + g_0[g_1 \otimes g_2 g_3 \otimes \cdots \otimes g_n] \pm \cdots)\\
                                                             &= [g_0 g_1 \otimes g_2 \otimes \cdots g_n] - [g_0 \otimes g_1 g_2 \otimes \cdots \otimes g_n] + [g_0 \otimes g_1 \otimes g_2 g_{3} \otimes \cdots \otimes g_n] \pm \cdots
.\end{align*}       

Other way around:
\begin{align*}
    d(s_{n-1}(g_0 [g_1 \otimes \cdots \otimes g_n]) &= d([g_0 \otimes g_1 \otimes \cdots  \otimes g_n])\\
                                                    &= g_0 [g_1 \otimes \cdots \otimes g_n]
                                                    - [g_0 g_1 \otimes \cdots \otimes g_n]
                                                    + [g_0 \otimes g_1 g_2 \otimes \cdots \otimes g_n]
                                                    - \cdots 
.\end{align*}
Adding the two yields
\[
    (ds + sd)(g_0 [g_1 \otimes \cdots \otimes g_n]) = g_0 [g_1 \otimes \cdots \otimes g_n]
.\] 
Done. 
Same proof for normalized.
\end{proof}


Now we use this to compute cohomology!

Start with projective resolution:
\[
    \to  B^u_3 
    \xrightarrow{d}  B_2
    \xrightarrow{d}  B_1
    \xrightarrow{d}  B_0
    \xrightarrow{\epsilon} \Z
    \to  0
.\] 

Delete and apply $\Hom_{\Z G}(-, A)$, swap arrows:
\[
    0
    \xrightarrow{ }  \Hom_{\Z G}( B_0,A)
    \xrightarrow{ }  \Hom_{\Z G}( B_1,A)
    \xrightarrow{ }  \Hom_{\Z G}( B_2,A)
    \to  \cdots
.\] 

Then $H^{n}(G, A)$ is the $n$-th cohomology group of this cochain complex.


\[
\Hom_{\Z G}(B_{n-1}^{u}, A) \xrightarrow{d^{*}} 
\Hom_{\Z G}(B_{n}^{u}, A) \xrightarrow{d^{*}} 
\Hom_{\Z G}(B_{n+1}^{u}, A) 
,\] 
where $d^{*} \phi = \phi  \circ  d$.

Now, $B_n^{u}$ is the free $\Z G$-modules on $[g_1 \otimes g_2 \otimes \cdots \otimes g_n]$.
So $\phi \in \Hom_{\Z G}(B_n^{u}, A)$ is completely determined by the generators.
And conversely, so
\[
    \Hom_{\Z G}(B_n^{u}, A) \leftrightarrow \{\phi  \mid \phi: G^{n} \to  A\} =: C^{n}(G, A)
.\] 
We call $C^{n}(G, A)$ the set of cochains of $G$ with coefficients in $A$.

\[
    \cdots \to  C^{n-1}(G, A) \to  
    C^{n}(G, A) \to  
    C^{n+1}(G, A) \to  \cdots
\] 

Let $\phi \in C^{n}(G, A)$. What is $d^{*}\phi \in C^{n+1}(G, A)$?
Well $d^{*}\phi = \phi  \circ  d$, so

\begin{align*}
    (d^{*} \phi)(g_1, g_2, \ldots, g_{n+1}) &= \phi d[g_1 \otimes \cdots g_{n+1}]\\
                                            &= 
                                            g_1 \phi(g_2, \ldots , g_n) 
                                            - \phi(g_1 g_2, g_3, \cdots, g_n)
                                            + \cdots \pm \phi(g_1, g_2, \cdots, g_{n-1})
.\end{align*} 

So then the cohomology is
\[
    \frac{\Ker d^{*}}{\im d^{*}} =: \frac{Z^{n}(G, A)}{B^{n}(G, A)}
,\] 
cocycles and coboundaries.


Let's do some calculations!

\[
    0 \to  C^{0}(G, A) \to  C^{1}(G, A) \to  C^{2}(G, A) \to  \cdots 
.\] 

\paragraph{Zeroth cohomology}
\begin{remark}
    $C^{0}(G, A) = \{f: G^{0} \to  A: [] \mapsto a\}  \cong A$.
\end{remark}

Now, what is the kernel? $\phi_a \in \Ker d$, where $d: C^{0} \to  C^{1}$.
So we require

\begin{align*}
    0 & = d \phi_a(g)\\
      &= \phi_a d([g])\\
      &= \phi_a (g[] - [])\\
      &= g \phi_a([]) - \phi_a([])\\
      &= ga - a
.\end{align*}
So $\phi_a \in  \Ker d$ iff $a \in A^{G}$.
So 
$Z^{0}(G, A) = A^{G}$ and $B^{0}(G, A) = 0$, so 
\[
    \boxed{H^{0}(G, A) = A^{G}}
.\] 
\paragraph{First cohomology}
We know that $C^{1}(G, A)  = \{f: G \to  A\} $.
So then 
\[
    Z^{1}(G, A) = \{f:G \to  A  \mid  df = 0\} 
.\] 
Then
\begin{align*}
    (df)(x, y) &= f  \circ  d[x \otimes y]\\
               &= f (x[y] - [xy] + [x])\\
               &= xf(y) - f(xy) + f(x)
.\end{align*} 
So $df = 0$ iff  $f(xy) = df(y) + f(x)$, so  $f$ is a derivation. 


Let $f \in C^{0}(G, A)$, so let $f = \phi_a$
Then \begin{align*}
    (df)(g)&= g f([]) - g([])\\
           &= ga - a
\end{align*}
So if $f$ corresponds to $a \in A$, then $df$ is a principal derivation.
So $B^{1}(G, A) = \PDer(G, A)$
\[
    \boxed{H^{1}(G, A) = \frac{\Der(G, A)}{\PDer(G, A)}}
.\] 

\paragraph{Second cohomology}

Let $f \in C^{2}(G, A)$.
Then $f \in Z^2(G, A) \iff df = 0$, so
\begin{align*}
    (df)(x,y,z) = xf(y,z) - f(xy,z) + f(x,yz) - f(x,y)
,\end{align*}
which we call the two cocycle condition.

$f \in B^2(G, A)$ if $f = dg$ for some  $g \in C^{1}(G, A)$.
Remember,
\[
    (dg)(x, y) = xg(y) - g(xy) + g(x)
.\] 

\begin{theorem}[6.5.8]
    Let $G$ be a finite group and $n = |G|$ 
    Then $n H^{i}(G, A) = 0$ for all $i > 0$.
\end{theorem}
\begin{remark}
    In book: proof that works in general, also for homology.
    Here, proof only works for cohomology (?) and we consider $H^2$ for simplicity.
\end{remark}
\begin{proof}
    Let $f \in Z^2(G, A)$,  so $f$ determines an element in  $H^2(G, A)$.
    Proof: $nf = d \lambda $ for some  $\lambda: G \to  A$.
    We define
    \[
        \lambda: G \to  A: x \mapsto \sum_{z \in G} f(x, z)
    .\] 
    Then
    \begin{align*}
        (d\lambda)(xy) &= d \lambda(y) \lambda(xy) + \lambda(x)\\
                       &= x \sum_z f(y,z) - \sum_z f(xy,z) + \sum_{z \in G} f(x,z)\\
                    &= x \sum_z f(y,z) - \sum_z f(xy,z) + \sum_{z \in G} f(x,yz)\\
    .\end{align*}
    Now we use the fact  that 
    \[
        0 = x f(y,z) - f(xy,z) + f(x,yz) - f(x,y)
    .\] 
    \begin{align*}
        &= x \sum_z f(y,z) - \sum_z f(xy,z) + \sum_{z \in G} f(x,yz) - \sum_z f(x,y) + \sum f(x,y)\\
        &= \sum_z (xf(y) f(xy,z) + f(x,yz) - f(x,y)) + \sum f(x,y)\\
        &= \sum_z f(x,y)\\
        d\lambda(x,y)&= |G| f(x,y)
    .\end{align*}
    Same proof works for all the cohomology groups.
\end{proof}

